simpler substs

pulse/lib/steel/pulse/Pulse.Prover.Substs.fsti
@@ -4,123 +4,181 @@ open FStar.List.Tot
 
 open Pulse.Syntax
 open Pulse.Typing.Env
+open Pulse.Typing
+open Pulse.Typing.Metatheory
 
 module L = FStar.List.Tot
 
-module RT = FStar.Reflection.Typing
-module T = FStar.Tactics
-
 module Env = Pulse.Typing.Env
 
-val t (g:env) : Type0
+type nt_substs = l:list subst_elt { forall elt. L.memP elt l ==> NT? elt }
 
-val as_subst (#g:env) (s:t g) : subst
+let compose_nt_substs (ss1 ss2:nt_substs) : nt_substs =
+  assume (forall elt. L.memP elt (ss1@ss2) <==> (L.memP elt ss1 \/ L.memP elt ss2));
+  ss1 @ ss2
 
-val as_map (#g:env) (s:t g) : Map.t var term
+let nt_subst_term (t:term) (ss:nt_substs) : term =
+  L.fold_left (fun t elt -> subst_term t [elt]) t ss
 
-let relates_to (g:env) (s:subst) (m:Map.t var term) =
-  (forall (elt:subst_elt).{:pattern L.memP elt s}
-          L.memP elt s ==> (NT? elt /\
-                            (let NT x t = elt in
-                             Map.contains m x /\
-                             Map.sel m x == t))) /\
+let nt_subst_st_term (t:st_term) (ss:nt_substs) : st_term =
+  L.fold_left (fun t elt -> subst_st_term t [elt]) t ss
+
+let nt_subst_comp (c:comp) (ss:nt_substs) : comp =
+  L.fold_left (fun c elt -> subst_comp c [elt]) c ss
+
+let nt_subst_env (g:env) (ss:nt_substs) : g':env { fstar_env g' == fstar_env g /\
+                                                   dom g' == dom g } =
+  admit ();
+  L.fold_left (fun g elt -> subst_env g [elt]) g ss
+
+val nt_subst_term_compose (t:term) (ss1 ss2:nt_substs)
+: Lemma (ensures nt_subst_term (nt_subst_term t ss1) ss2 ==
+                 nt_subst_term t (compose_nt_substs ss1 ss2))
+
+val nt_subst_st_term_compose (t:st_term) (ss1 ss2:nt_substs)
+: Lemma (ensures nt_subst_st_term (nt_subst_st_term t ss1) ss2 ==
+                 nt_subst_st_term t (compose_nt_substs ss1 ss2))
+
+val nt_subst_comp_compose (c:comp) (ss1 ss2:nt_substs)
+: Lemma (ensures nt_subst_comp (nt_subst_comp c ss1) ss2 ==
+                 nt_subst_comp c (compose_nt_substs ss1 ss2))
+
+let rec well_typed_ss (g:env) (uvs:env) (ss:nt_substs) : Tot Type0 (decreases L.length ss) =
+  match bindings uvs, ss with
+  | [], [] -> True
+  | _::_, (NT x e)::ss_rest ->
+    let y, ty, rest_uvs = remove_binding uvs in
+    x == y /\
+    tot_typing g e ty /\
+    well_typed_ss g (subst_env rest_uvs [ NT x e ]) ss_rest
+  | _, _ -> False
+
+val st_typing_nt_substs
+  (g:env) (uvs:env) (g':env { pairwise_disjoint g uvs g' })
+  (#t:st_term) (#c:comp_st) (t_typing:st_typing (push_env g (push_env uvs g')) t c)
+  (ss:nt_substs { well_typed_ss g uvs ss })
+: st_typing (push_env g (nt_subst_env g' ss)) (nt_subst_st_term t ss) (nt_subst_comp c ss)
+
+val vprop_equiv_nt_substs
+  (g:env) (uvs:env) (g':env { pairwise_disjoint g uvs g' })
+  (#p1 #p2:vprop) (veq:vprop_equiv (push_env g (push_env uvs g')) p1 p2)
+  (ss:nt_substs { well_typed_ss g uvs ss })
+: vprop_equiv (push_env g (nt_subst_env g' ss)) (nt_subst_term p1 ss) (nt_subst_term p2 ss)
+
+
+val t : Type0
+
+val as_nt_substs (s:t) : nt_substs
+
+val as_map (s:t) : Map.t var term
+
+// let relates_to (g:env) (s:subst) (m:Map.t var term) =
+//   (forall (elt:subst_elt).{:pattern L.memP elt s}
+//           L.memP elt s ==> (NT? elt /\
+//                             (let NT x t = elt in
+//                              Map.contains m x /\
+//                              Map.sel m x == t))) /\
   
-  (forall (x:var).{:pattern Map.contains m x}
-                  Map.contains m x ==> (L.memP (NT x (Map.sel m x)) s)) /\
+//   (forall (x:var).{:pattern Map.contains m x}
+//                   Map.contains m x ==> (L.memP (NT x (Map.sel m x)) s)) /\
 
-  (forall (x:var).{:pattern Map.contains m x}
-                  Map.contains m x ==> ((~ (Set.mem x (dom g))) /\
-                                        freevars (Map.sel m x) `Set.subset` dom g))
+//   (forall (x:var).{:pattern Map.contains m x}
+//                   Map.contains m x ==> ((~ (Set.mem x (dom g))) /\
+//                                         freevars (Map.sel m x) `Set.subset` dom g))
 
-val subst_as_map (#g:env) (s:t g)
-  : Lemma (relates_to g (as_subst s) (as_map s))
-          [SMTPat (as_subst s); SMTPat (as_map s)]
+// val subst_as_map (#g:env) (s:t g)
+//   : Lemma (relates_to g (as_subst s) (as_map s))
+//           [SMTPat (as_subst s); SMTPat (as_map s)]
 
-let dom (#g:_) (s:t g) : Set.set var = Map.domain (as_map s)
+let dom (s:t) : Set.set var = Map.domain (as_map s)
 
-let lookup (#g:_) (s:t g) (x:var { x `Set.mem` dom s }) : term =
-  Map.sel (as_map s) x
+// let lookup (#g:_) (s:t g) (x:var { x `Set.mem` dom s }) : term =
+//   Map.sel (as_map s) x
 
-let equal (#g:env) (s1 s2:t g) =
-  Set.equal (dom s1) (dom s2) /\
-  (forall (x:var).{:pattern Set.mem x (dom s1)} Set.mem x (dom s1) ==> lookup s1 x == lookup s2 x)
+// let equal (#g:env) (s1 s2:t g) =
+//   Set.equal (dom s1) (dom s2) /\
+//   (forall (x:var).{:pattern Set.mem x (dom s1)} Set.mem x (dom s1) ==> lookup s1 x == lookup s2 x)
 
-val equal_elim (#g:_) (s1 s2:t g)
-  : Lemma (requires equal s1 s2)
-          (ensures s1 == s2)
-          [SMTPat (equal s1 s2)]
+// val equal_elim (#g:_) (s1 s2:t g)
+//   : Lemma (requires equal s1 s2)
+//           (ensures s1 == s2)
+//           [SMTPat (equal s1 s2)]
 
-val empty (g:env) : t g
+val empty : t
 
-val empty_dom (g:_)
-  : Lemma (dom (empty g) == Set.empty)
-          [SMTPat (dom (empty g))]
+val empty_dom (_:unit)
+  : Lemma (dom empty == Set.empty)
 
-val singleton (g:env)
-  (x:var { ~ (Set.mem x (Env.dom g)) })
-  (e:term { freevars e `Set.subset` Env.dom g })
-  : t g
+// val singleton (g:env)
+//   (x:var { ~ (Set.mem x (Env.dom g)) })
+//   (e:term { freevars e `Set.subset` Env.dom g })
+//   : t g
 
-val singleton_dom (#g:_)
-  (x:var { ~ (Set.mem x (Env.dom g)) })
-  (e:term { freevars e `Set.subset` Env.dom g })
-  : Lemma (ensures dom (singleton g x e) == Set.singleton x)
-          [SMTPat (dom (singleton g x e))]
+// val singleton_dom (#g:_)
+//   (x:var { ~ (Set.mem x (Env.dom g)) })
+//   (e:term { freevars e `Set.subset` Env.dom g })
+//   : Lemma (ensures dom (singleton g x e) == Set.singleton x)
+//           [SMTPat (dom (singleton g x e))]
 
-val push (#g:_) (s1:t g) (s2:t g { Set.disjoint (dom s1) (dom s2)})
-  : t g
+val push (s1:t) (s2:t { Set.disjoint (dom s1) (dom s2)})
+  : t
 
-val push_substs_as_map (#g:_) (s1 s2:t g)
+val push_as_map (s1 s2:t)
   : Lemma (requires Set.disjoint (dom s1) (dom s2))
           (ensures as_map (push s1 s2) == Map.concat (as_map s1) (as_map s2))
           [SMTPat (as_map (push s1 s2))]
 
-let subst_extends (#g:_) (s1 s2:t g) =
-  exists s3. s1 == push s2 s3
+// val push_substs_as_map (#g:_) (s1 s2:t g)
+//   : Lemma (requires Set.disjoint (dom s1) (dom s2))
+//           (ensures as_map (push s1 s2) == Map.concat (as_map s1) (as_map s2))
+//           [SMTPat (as_map (push s1 s2))]
 
-let subst_term (#g:_) (s:t g) (t:term) =
-  subst_term t (as_subst s)
+// let subst_extends (#g:_) (s1 s2:t g) =
+//   exists s3. s1 == push s2 s3
 
-let subst_st_term (#g:_) (s:t g) (t:st_term) =
-  subst_st_term t (as_subst s)
+// let subst_term (#g:_) (s:t g) (t:term) =
+//   subst_term t (as_subst s)
 
-let subst_comp (#g:_) (s:t g) (c:comp) =
-  subst_comp c (as_subst s)
+// let subst_st_term (#g:_) (s:t g) (t:st_term) =
+//   subst_st_term t (as_subst s)
 
-val push_subst_term (#g:_) (s1 s2:t g) (t:term)
-  : Lemma (requires Set.disjoint (dom s1) (dom s2))
-          (ensures subst_term (push s1 s2) t ==
-                   subst_term s2 (subst_term s1 t))
-          [SMTPat (subst_term s2 (subst_term s1 t))]
+// let subst_comp (#g:_) (s:t g) (c:comp) =
+//   subst_comp c (as_subst s)
 
-val push_subst_st_term (#g:_) (s1 s2:t g) (t:st_term)
-  : Lemma (requires Set.disjoint (dom s1) (dom s2))
-          (ensures subst_st_term (push s1 s2) t ==
-                   subst_st_term s2 (subst_st_term s1 t))
-          [SMTPat (subst_st_term s2 (subst_st_term s1 t))]
+// val push_subst_term (#g:_) (s1 s2:t g) (t:term)
+//   : Lemma (requires Set.disjoint (dom s1) (dom s2))
+//           (ensures subst_term (push s1 s2) t ==
+//                    subst_term s2 (subst_term s1 t))
+//           [SMTPat (subst_term s2 (subst_term s1 t))]
 
-val push_subst_comp (#g:_) (s1 s2:t g) (c:comp)
-  : Lemma (requires Set.disjoint (dom s1) (dom s2))
-          (ensures subst_comp (push s1 s2) c ==
-                   subst_comp s2 (subst_comp s1 c))
-          [SMTPat (subst_comp s2 (subst_comp s1 c))]
+// val push_subst_st_term (#g:_) (s1 s2:t g) (t:st_term)
+//   : Lemma (requires Set.disjoint (dom s1) (dom s2))
+//           (ensures subst_st_term (push s1 s2) t ==
+//                    subst_st_term s2 (subst_st_term s1 t))
+//           [SMTPat (subst_st_term s2 (subst_st_term s1 t))]
 
-val subst_closed_term (#g:_) (s:t g) (t:term)
-  : Lemma (requires freevars t `Set.subset` Env.dom g)
-          (ensures subst_term s t == t)
+// val push_subst_comp (#g:_) (s1 s2:t g) (c:comp)
+//   : Lemma (requires Set.disjoint (dom s1) (dom s2))
+//           (ensures subst_comp (push s1 s2) c ==
+//                    subst_comp s2 (subst_comp s1 c))
+//           [SMTPat (subst_comp s2 (subst_comp s1 c))]
 
-val subst_closed_st_term (#g:_) (s:t g) (t:st_term)
-  : Lemma (requires freevars_st t `Set.subset` Env.dom g)
-          (ensures subst_st_term s t == t)
+// val subst_closed_term (#g:_) (s:t g) (t:term)
+//   : Lemma (requires freevars t `Set.subset` Env.dom g)
+//           (ensures subst_term s t == t)
 
-val subst_closed_comp (#g:_) (s:t g) (c:comp)
-  : Lemma (requires freevars_comp c `Set.subset` Env.dom g)
-          (ensures subst_comp s c == c)
+// val subst_closed_st_term (#g:_) (s:t g) (t:st_term)
+//   : Lemma (requires freevars_st t `Set.subset` Env.dom g)
+//           (ensures subst_st_term s t == t)
 
-val diff (#g:_) (s1:t g) (s2:t g { Set.subset (dom s2) (dom s1) })
-  : s3:t g { Set.disjoint (dom s3) (dom s2) }
+// val subst_closed_comp (#g:_) (s:t g) (c:comp)
+//   : Lemma (requires freevars_comp c `Set.subset` Env.dom g)
+//           (ensures subst_comp s c == c)
 
-val diff_push (#g:_) (s1 s2:t g)
-  : Lemma (requires Set.subset (dom s2) (dom s1))
-          (ensures push (diff s1 s2) s2 == s1)
-          [SMTPat (diff s1 s2)]
+// val diff (#g:_) (s1:t g) (s2:t g { Set.subset (dom s2) (dom s1) })
+//   : s3:t g { Set.disjoint (dom s3) (dom s2) }
+
+// val diff_push (#g:_) (s1 s2:t g)
+//   : Lemma (requires Set.subset (dom s2) (dom s1))
+//           (ensures push (diff s1 s2) s2 == s1)
+//           [SMTPat (diff s1 s2)]
