pulse/lib/steel/pulse/Pulse.Prover.Util.fsti
@@ -4,108 +4,10 @@ open FStar.List.Tot
 
 open Pulse.Syntax
 open Pulse.Typing
-open Pulse.Checker.Common
 open Pulse.Typing.Metatheory
-open Pulse.Checker.VPropEquiv
 
 module L = FStar.List.Tot
-module T = FStar.Tactics
-module RT = FStar.Reflection.Typing
-module Psubst = Pulse.Prover.Substs
 
-type nt_substs = l:list subst_elt { forall elt. L.memP elt l ==> NT? elt }
-
-let compose_nt_substs (ss1 ss2:nt_substs) : nt_substs =
-  assume (forall elt. L.memP elt (ss1@ss2) <==> (L.memP elt ss1 \/ L.memP elt ss2));
-  ss1 @ ss2
-
-let nt_subst_term (t:term) (ss:nt_substs) : term =
-  L.fold_left (fun t elt -> subst_term t [elt]) t ss
-
-let nt_subst_st_term (t:st_term) (ss:nt_substs) : st_term =
-  L.fold_left (fun t elt -> subst_st_term t [elt]) t ss
-
-let nt_subst_comp (c:comp) (ss:nt_substs) : comp =
-  L.fold_left (fun c elt -> subst_comp c [elt]) c ss
-
-let nt_subst_env (g:env) (ss:nt_substs) : g':env { fstar_env g' == fstar_env g /\
-                                                   dom g' == dom g } =
-  admit ();
-  L.fold_left (fun g elt -> subst_env g [elt]) g ss
-
-let rec nt_subst_term_compose (t:term) (ss1 ss2:nt_substs)
-: Lemma (ensures nt_subst_term (nt_subst_term t ss1) ss2 ==
-                 nt_subst_term t (compose_nt_substs ss1 ss2))
-        (decreases L.length ss1) =
-
-match ss1 with
-| [] -> ()
-| (NT x e)::tl -> nt_subst_term_compose (subst_term t [ NT x e ]) tl ss2
-
-let rec nt_subst_st_term_compose (t:st_term) (ss1 ss2:nt_substs)
-: Lemma (ensures nt_subst_st_term (nt_subst_st_term t ss1) ss2 ==
-                 nt_subst_st_term t (compose_nt_substs ss1 ss2))
-        (decreases L.length ss1) =
-
-match ss1 with
-| [] -> ()
-| (NT x e)::tl -> nt_subst_st_term_compose (subst_st_term t [ NT x e ]) tl ss2
-
-let rec nt_subst_comp_compose (c:comp) (ss1 ss2:nt_substs)
-: Lemma (ensures nt_subst_comp (nt_subst_comp c ss1) ss2 ==
-                 nt_subst_comp c (compose_nt_substs ss1 ss2))
-        (decreases L.length ss1) =
-
-match ss1 with
-| [] -> ()
-| (NT x e)::tl -> nt_subst_comp_compose (subst_comp c [ NT x e ]) tl ss2
-
-let rec well_typed_ss (g:env) (uvs:env) (ss:nt_substs) : Tot Type0 (decreases L.length ss) =
-  match bindings uvs, ss with
-  | [], [] -> True
-  | _::_, (NT x e)::ss_rest ->
-    let y, ty, rest_uvs = remove_binding uvs in
-    x == y /\
-    tot_typing g e ty /\
-    well_typed_ss g (subst_env rest_uvs [ NT x e ]) ss_rest
-  | _, _ -> False
-
-
-let coerce_eq (#a #b:Type) (x:a) (_:squash (a === b)) : y:b{y == x} = x
-
-let rec st_typing_nt_substs
-  (g:env) (uvs:env) (g':env { pairwise_disjoint g uvs g' })
-  (#t:st_term) (#c:comp_st) (t_typing:st_typing (push_env g (push_env uvs g')) t c)
-  (ss:nt_substs { well_typed_ss g uvs ss })
-: Tot (st_typing (push_env g (nt_subst_env g' ss)) (nt_subst_st_term t ss) (nt_subst_comp c ss))
-      (decreases L.length ss) =
-
-match bindings uvs with
-| [] ->
-  assert (equal (push_env uvs g') g');
-  t_typing
-
-| _ ->
-  let x, ty, uvs' = remove_binding uvs in
-  let (NT y e)::ss' = ss in
-  let e_typing = FStar.IndefiniteDescription.elim_squash #(tot_typing g e ty) () in
-  push_env_assoc (singleton_env (fstar_env uvs) x ty) uvs' g';
-  let t_typing
-    : st_typing (push_env g (push_env (singleton_env (fstar_env g) x ty) (push_env uvs' g'))) t c
-    = coerce_eq t_typing () in
-  let t_typing
-    : st_typing (push_env g (subst_env (push_env uvs' g') [ NT y e ]))
-                (subst_st_term t [ NT y e ])
-                (subst_comp c [ NT y e ])
-    = st_typing_subst g x ty (push_env uvs' g') e_typing t_typing in
-
-  assume (subst_env (push_env uvs' g') [ NT y e ] ==
-          push_env (subst_env uvs' [ NT y e ]) (subst_env g' [ NT y e ]));
-
-  st_typing_nt_substs g
-    (subst_env uvs' [ NT y e ])
-    (subst_env g' [ NT y e ])
-    t_typing ss'
 
 
 
